Up-to-date version, includes a (partial) example.

comp_langLib.sig
@@ -1,0 +1,8 @@
+signature comp_langLib =
+sig
+
+    include Abbrev
+
+    val define_compiler_exp   : string -> term -> thm
+
+end
