comp_langScript.sml
@@ -21,22 +21,28 @@ val _ = Hol_datatype `
            | WORD_IMM of word32                       (* any constant 32-bit word *)
            | WORD_LSL of WORD_EXP => num              (* left-shift *)
            | WORD_LSR of WORD_EXP => num              (* right-shift *)
-           | WORD_MASK of WORD_EXP => word32          (* word and with immediate *)
-           | WORD_BIT_CLEAR of WORD_EXP => num        (* set bit i to F *)
-           | WORD_BIT_SET of WORD_EXP => num          (* set bit i to T *)
-           | WORD_BIT_COPY of WORD_EXP => num => num  (* copy bit from instruction *)
-           | WORD_SIGN_EXTEND of WORD_EXP => num`;    (* sign-extend from bit i *)
+           | WORD_AND of WORD_EXP => word32           (* word and with immediate *)
+           | WORD_OR of WORD_EXP => word32            (* word or with immediate *)
+           | WORD_BITS of WORD_EXP => num => num      (* or bits from instruction *)
+           | WORD_SIGN_EXTEND of WORD_EXP => num      (* sign-extend from bit i *)
+           | WORD_ROTATE of WORD_EXP => num           (* special word rotate right *)`;
+
+val sign_extend_def = Define `
+  sign_extend n (w:'a word) = w << (dimword(:'a) - n) >> (dimword(:'a) - n)`;
+
+val arm_immediate_rotate_def = Define `
+  arm_immediate_rotate n (w:word32) (e:word32) = e #>> (2 * w2n (w >> n && 15w))`;
 
 val eval_word_exp_def = Define `
   (eval_word_exp w (WORD_INSTRUCTION) = w) /\
   (eval_word_exp w (WORD_IMM x) = x) /\
   (eval_word_exp w (WORD_LSR e n) = eval_word_exp w e >>> n) /\
   (eval_word_exp w (WORD_LSL e n) = eval_word_exp w e << n) /\
-  (eval_word_exp w (WORD_MASK e x) = eval_word_exp w e && x) /\
-  (eval_word_exp w (WORD_BIT_CLEAR e i) = (i :+ F) (eval_word_exp w e)) /\
-  (eval_word_exp w (WORD_BIT_SET e i) = (i :+ T) (eval_word_exp w e)) /\
-  (eval_word_exp w (WORD_BIT_COPY e i j) = (j :+ w ' i) (eval_word_exp w e)) /\
-  (eval_word_exp w (WORD_SIGN_EXTEND e n) = (eval_word_exp w e) << (32 - n) >> (32 - n))`;
+  (eval_word_exp w (WORD_AND e x) = eval_word_exp w e && x) /\
+  (eval_word_exp w (WORD_OR e x) = eval_word_exp w e || x) /\
+  (eval_word_exp w (WORD_BITS e i j) = eval_word_exp w e || (i -- j) w) /\
+  (eval_word_exp w (WORD_SIGN_EXTEND e n) = sign_extend n (eval_word_exp w e)) /\
+  (eval_word_exp w (WORD_ROTATE e n) = arm_immediate_rotate n w (eval_word_exp w e))`;
 
 val e2n_def = Define `e2n w e = w2n (eval_word_exp w e)`;
 val e2w_def = Define `e2w w e = w2w (eval_word_exp w e)`;
@@ -47,8 +53,8 @@ val e2b_def = Define `e2b w e = (eval_word_exp w e) ' 0`;
 
 val _ = Hol_datatype `
   EMIT_EXP =
-      EMIT_CONDITIONAL of WORD_EXP
-    | EMIT_MARKER 
+      EMIT_CONDITIONAL of WORD_EXP => WORD_EXP
+    | EMIT_MARKER
     | EMIT_ASSERT of WORD_EXP
     | EMIT_MOVE of WORD_EXP => WORD_EXP
     | EMIT_IMM of WORD_EXP => WORD_EXP
@@ -56,12 +62,13 @@ val _ = Hol_datatype `
     | EMIT_REG_WRITE of WORD_EXP => WORD_EXP
     | EMIT_MEM_BYTE_READ of WORD_EXP
     | EMIT_MEM_WORD_READ of WORD_EXP
-    | EMIT_MEM_BYTE_WRITE of WORD_EXP  
+    | EMIT_MEM_BYTE_WRITE of WORD_EXP
     | EMIT_MEM_WORD_WRITE of WORD_EXP
+    | EMIT_ADD_IMM of WORD_EXP => WORD_EXP
     | EMIT_BINOP of WORD_EXP => WORD_EXP`;
 
 val eval_emit_exp_def = Define `
-  (eval_emit_exp w (EMIT_CONDITIONAL w1) = MINI_CONDITIONAL (e2w w w1)) /\
+  (eval_emit_exp w (EMIT_CONDITIONAL w1 w2) = MINI_CONDITIONAL (e2w w w1) (e2w w w2)) /\
   (eval_emit_exp w (EMIT_MARKER) = MINI_MARKER) /\
   (eval_emit_exp w (EMIT_ASSERT w1) = MINI_ASSERT (num2assert (e2n w w1))) /\
   (eval_emit_exp w (EMIT_MOVE w1 w2) = MINI_MOVE (e2w w w1) (e2w w w2)) /\
@@ -72,6 +79,7 @@ val eval_emit_exp_def = Define `
   (eval_emit_exp w (EMIT_MEM_WORD_READ w1) = MINI_MEM_WORD_READ (e2w w w1)) /\
   (eval_emit_exp w (EMIT_MEM_BYTE_WRITE w1) = MINI_MEM_BYTE_WRITE (e2w w w1)) /\
   (eval_emit_exp w (EMIT_MEM_WORD_WRITE w1) = MINI_MEM_WORD_WRITE (e2w w w1)) /\
+  (eval_emit_exp w (EMIT_ADD_IMM w1 w2) = MINI_ADD_IMM (e2w w w1) (e2w w w2)) /\
   (eval_emit_exp w (EMIT_BINOP w1 w2) = MINI_BINOP (num2binop (e2n w w1)) (e2b w w2))`;
 
 
@@ -87,6 +95,9 @@ val _ = Hol_datatype `
     | COMPILER_TRY of COMPILER_EXP => COMPILER_EXP
     | COMPILER_EMIT of EMIT_EXP`;
 
+val compiler_try_def = Define `
+  compiler_try x y = let res = x in if res = [] then y else res`;
+
 val eval_compiler_exp_def = Define `
   (eval_compiler_exp w (COMPILER_SKIP) = []) /\
   (eval_compiler_exp w (COMPILER_SEQ x y) =
@@ -95,8 +106,7 @@ val eval_compiler_exp_def = Define `
      if eval_word_exp w e = w1 then eval_compiler_exp w x
                                else eval_compiler_exp w y) /\
   (eval_compiler_exp w (COMPILER_TRY x y) =
-     let res = eval_compiler_exp w x in
-       if res = [] then eval_compiler_exp w y else res) /\
+     compiler_try (eval_compiler_exp w x) (eval_compiler_exp w y)) /\
   (eval_compiler_exp w (COMPILER_EMIT z) = [eval_emit_exp w z])`;
 
 
@@ -114,20 +124,25 @@ val ARM_OK_def = Define `
     ~(ARM_READ_STATUS psrT state) /\ ~(ARM_READ_STATUS psrE state) /\
     (ARM_MODE state = 16w)`;
 
+val ARM_ERASE_ACCESSES_def = Define `
+  ARM_ERASE_ACCESSES s = s with accesses := []`;
+
 val COMP_CORRECT_def = Define `
   COMP_CORRECT compiler =
     !instr. let code = eval_compiler_exp instr compiler in
-              if code = [] then T else 
-                !regs ok s. let (regs1,ok1,s1) = eval_mini_list code (regs,ok,s) in
-                              (ARM_READ_MEM_WORD (ARM_READ_REG 15w s) s = instr) /\
-                              aligned (ARM_READ_REG 15w s,2) /\ ARM_OK s /\ ok1 ==> 
-                              (ARM_NEXT NoInterrupt s = SOME s1) /\ ARM_OK s1`;
+              (code = []) \/
+              !regs ok s. let (regs1,ok1,s1) = eval_mini_list code (regs,ok,s) in
+                            (ARM_READ_MEM_WORD (ARM_READ_REG 15w s) s = instr) /\
+                            aligned (ARM_READ_REG 15w s,2) /\ ARM_OK s /\ ok1 ==>
+                            ?s2. (ARM_NEXT NoInterrupt s = SOME s2) /\ ARM_OK s2 /\
+                                 (ARM_ERASE_ACCESSES s1 = ARM_ERASE_ACCESSES s2)`;
 
 (* This property can be decomposed across COMPILER_TRY. *)
 
 val COMP_CORRECT_TRY = store_thm("COMP_CORRECT_TRY",
   ``!x y. COMP_CORRECT x /\ COMP_CORRECT y ==> COMP_CORRECT (COMPILER_TRY x y)``,
-  SIMP_TAC std_ss [COMP_CORRECT_def,eval_compiler_exp_def,LET_DEF] THEN METIS_TAC []);
+  SIMP_TAC std_ss [COMP_CORRECT_def,eval_compiler_exp_def,
+     LET_DEF,compiler_try_def] THEN METIS_TAC []);
 
 (* The NOT_IMPLEMENTED assertion is always a correct compilation. *)
 
