comp_exampleScript.sml
@@ -1,0 +1,148 @@
+
+open HolKernel Parse boolLib bossLib; val _ = new_theory "comp_example";
+
+open mini_langTheory comp_langTheory comp_langLib;
+
+open wordsTheory wordsLib listTheory arithmeticTheory;
+open arm_decoderTheory arm_opsemTheory arm_coretypesTheory armTheory armLib;
+open arm_stepTheory arm_seq_monadTheory arm_encoderLib;
+
+
+infix \\
+val op \\ = op THEN
+
+
+(* We start by defining a compiler that can produce MINI code for
+   <data><cond> rd,rn,#<immediate>. The following is the encoding we
+   compile. *)
+
+val arm_data_imm_enc_tm =
+  ``((1w << 25
+      || w2w (opcode:word4) << 21
+      || w2w (rn:word4) << 16
+      || w2w (rd:word4) << 12
+      || w2w (rotate_imm:word4) << 8
+      || w2w (imm8:word8)
+      || w2w (s:word1) << 20
+      || w2w (cond:word4) << 28)):word32``
+
+val cond_bits = ``(31 -- 28):word32->word32``
+val opcode_bits = ``(24 -- 21):word32->word32``
+val rn_bits = ``(19 -- 16):word32->word32``
+val rd_bits = ``(15 -- 12):word32->word32``
+val imm8_bits = ``(7 -- 0):word32->word32``
+val rotate_imm_bits = ``(11 -- 8):word32->word32``
+val s_bit = ``(w:word32) ' 20``
+
+val select_lemma = blastLib.BBLAST_PROVE
+  ``(^cond_bits ^arm_data_imm_enc_tm = w2w cond) /\
+    (^opcode_bits ^arm_data_imm_enc_tm = w2w opcode) /\
+    (^rn_bits ^arm_data_imm_enc_tm = w2w rn) /\
+    (^rd_bits ^arm_data_imm_enc_tm = w2w rd) /\
+    (^imm8_bits ^arm_data_imm_enc_tm = w2w imm8) /\
+    (^rotate_imm_bits ^arm_data_imm_enc_tm = w2w rotate_imm) /\
+    (^arm_data_imm_enc_tm ' 20 = (s:word1) ' 0)``
+
+val w2w_lemma = blastLib.BBLAST_PROVE
+  ``(w2w ((w2w w8):word32) = w8:word8) /\
+    (w2w ((w2w w4):word32) = w4:word4) /\
+    (w2w ((w2w w2):word32) = w2:word2)``
+
+
+(* The mask with which we identify this instruction *)
+
+fun max_words tm = let
+  fun max_word v = let
+    val ty = type_of v |> dest_type |> snd |> last
+    in v |-> (wordsSyntax.mk_word_sub(wordsSyntax.mk_n2w(``0:num``,ty),
+                                      wordsSyntax.mk_n2w(``1:num``,ty))
+              |> EVAL |> concl |> rand) end
+    handle HOL_ERR _ => ``v:num`` |-> ``v:num``
+  in subst (map (max_word) (free_vars tm)) tm end
+
+val mask = (rand o concl o EVAL)
+  (wordsSyntax.mk_word_1comp(max_words arm_data_imm_enc_tm))
+
+fun zero_words tm = let
+  fun zero_word v = let
+    val ty = type_of v |> dest_type |> snd |> last
+    in v |-> wordsSyntax.mk_n2w(``0:num``,ty) end
+    handle HOL_ERR _ => ``v:num`` |-> ``v:num``
+  in subst (map (zero_word) (free_vars tm)) tm end
+
+val match = (rand o concl o EVAL) (zero_words arm_data_imm_enc_tm)
+
+(* We prove that the mask is suffient. *)
+
+val tm = list_mk_exists(free_vars arm_data_imm_enc_tm,``w = ^arm_data_imm_enc_tm``)
+val tm = ``!w. ((w:word32) && ^mask = ^match) ==> ^tm``
+(* This would have been a pain to prove without blast! *)
+val mask_lemma = blastLib.BBLAST_PROVE tm
+
+
+(* We use define_compiler_exp to define the compiling function. *)
+
+val data_imm_compiler_thm = define_compiler_exp "data_imm_compiler"
+  ``if (w:word32) && ^mask = ^match then
+      if ^cond_bits w = 15w then (* cond must not be 15w *)
+        [MINI_ASSERT ASSERT_UNPREDICTABLE]
+      else
+        (* check for conditional execution *)
+        (if ^cond_bits w = 14w then [] else [MINI_CONDITIONAL (w2w (^cond_bits w)) 4w])
+        ++
+        (* bump pc forward *)
+        [MINI_REG_READ 3w 15w;
+         MINI_ADD_IMM 3w 4w;
+         MINI_REG_WRITE 15w 3w]
+        ++
+        (* perform core operation *)
+        [MINI_REG_READ 0w (w2w (^rn_bits w))] ++
+        (if ^rn_bits w = 15w then [MINI_ADD_IMM 0w 4w] else []) ++
+        [MINI_IMM 1w (arm_immediate_rotate 8 w (^imm8_bits w))] ++
+        (if ^opcode_bits w = 4w then
+           [MINI_BINOP BINOP_ADD ^s_bit]
+         else if ^opcode_bits w = 2w then
+           [MINI_BINOP BINOP_SUB ^s_bit]
+         else
+           [MINI_ASSERT ASSERT_NOT_IMPLEMENTED]) ++
+        [MINI_REG_WRITE (w2w (^rd_bits w)) 0w]
+    else []``
+
+(* Note that the resulting data_imm_compiler_thm is of the form:
+
+     eval_compiler_exp w data_imm_compiler =
+       if (w:word32) && ^mask = ^match then ... else ...
+
+   The define_compiler_exp function generates a deep embedding which
+   it defines to have the given name, in this case "add_imm_compiler".
+   The deep embedding is defined so that it has exactly the semantics
+   of the supplied term (w.r.t. eval_compiler_exp). In other words,
+   the user need never deal with the verbose deep embedding
+   directly. If you're curious, type
+
+     fetch "-" "data_imm_compiler"
+
+   to see the deep embedding. *)
+
+
+(* Now let's attempt to prove that this complier is correct. *)
+
+val select_lemma2 = blastLib.BBLAST_PROVE
+  ``(^arm_data_imm_enc_tm >> 8 && 15w) = w2w rotate_imm``
+
+val (CHEAT_TAC:tactic) = fn x => ([],fn t => mk_thm x);
+
+val data_imm_compiler_correct = store_thm("data_imm_compiler_correct",
+  ``COMP_CORRECT data_imm_compiler``,
+  SIMP_TAC std_ss [COMP_CORRECT_def,data_imm_compiler_thm,Once LET_DEF]
+  \\ STRIP_TAC \\ REVERSE (Cases_on `(instr:word32) && ^mask = ^match`)
+  THEN1 (FULL_SIMP_TAC std_ss []) \\ FULL_SIMP_TAC std_ss [] \\ DISJ2_TAC
+  \\ IMP_RES_TAC mask_lemma \\ ASM_REWRITE_TAC [select_lemma,w2w_lemma]
+  \\ Cases_on `w2w cond = 15w:word32` \\ FULL_SIMP_TAC std_ss []
+  THEN1 (FULL_SIMP_TAC std_ss [eval_mini_list_def,LET_DEF,eval_mini_def,check_assert_def])
+  \\ ASM_SIMP_TAC std_ss [select_lemma2,arm_immediate_rotate_def]
+  (* ... *)
+  \\ CHEAT_TAC);
+
+
+val _ = export_theory();
