mini_langScript.sml
@@ -22,10 +22,10 @@ val _ = type_abbrev("mini_state",``:(mini_reg -> word32) # bool # arm_state``);
 (* === abstract syntax === *)
 
 val _ = Hol_datatype `
-  BINOP = BINOP_ADD 
-        | BINOP_SUB 
-        | BINOP_OR 
-        | BINOP_XOR 
+  BINOP = BINOP_ADD
+        | BINOP_SUB
+        | BINOP_OR
+        | BINOP_XOR
         | BINOP_AND`;
         (* TST and CMP not needed, since AND and SUB suffice *)
 
@@ -39,7 +39,7 @@ val _ = Hol_datatype `
   MINI_INSTRUCTION =
 
     (* execute NOP and skip to next MINI_MARKER, in case condition not met *)
-      MINI_CONDITIONAL of word4
+      MINI_CONDITIONAL of word4 => word32
     | MINI_MARKER (* execution of this has no effect *)
 
     (* assertions *)
@@ -60,6 +60,7 @@ val _ = Hol_datatype `
     | MINI_MEM_WORD_WRITE of word32   (* memory[A+imm32] := B *)
 
     (* arithmetic/logic *)
+    | MINI_ADD_IMM of word2 => word32 (* simple addition, e.g. for pc update *)
     | MINI_BINOP of BINOP => bool (* "s-flag" as in adds vs add *)
    (* MINI_MONOPs not needed as NOT x is XOR x 0w and NEG r is SUB 0, r *)`;
 
@@ -72,12 +73,20 @@ val num2binop_def = Define `
     if n = 3 then BINOP_XOR else
     if n = 4 then BINOP_AND else BINOP_ADD`;
 
+val num2binop_thm = save_thm("num2binop_thm",
+  find_terms (numSyntax.is_numeral) (concl num2binop_def) |> rev
+  |> map (fn tm => EVAL (``num2binop ^tm``)) |> LIST_CONJ);
+
 val num2assert_def = Define `
-  num2assert n = 
+  num2assert n =
     if n = 0 then ASSERT_NOT_IMPLEMENTED else
     if n = 1 then ASSERT_UNPREDICTABLE else
     if n = 2 then ASSERT_ALIGNED_HALF else
     if n = 3 then ASSERT_ALIGNED_WORD else ASSERT_UNPREDICTABLE`;
+
+val num2assert_thm = save_thm("num2assert_thm",
+  find_terms (numSyntax.is_numeral) (concl num2assert_def) |> rev
+  |> map (fn tm => EVAL (``num2assert ^tm``)) |> LIST_CONJ);
 
 
 (* === semantics === *)
@@ -101,27 +110,27 @@ val arm_condition_passed_def = Define `
        result`;
 
 val ARM_READ_MEM_WORD_def = Define `
-  ARM_READ_MEM_WORD a s = 
-    word32 [ARM_READ_MEM a s; ARM_READ_MEM (a+1w) s; 
+  ARM_READ_MEM_WORD a s =
+    word32 [ARM_READ_MEM a s; ARM_READ_MEM (a+1w) s;
             ARM_READ_MEM (a+2w) s; ARM_READ_MEM (a+3w) s]`;
 
 val ARM_WRITE_MEM_WORD_def = Define `
-  ARM_WRITE_MEM_WORD a w s = 
+  ARM_WRITE_MEM_WORD a w s =
     let bs = bytes (w,4) in
-      (ARM_WRITE_MEM a (EL 0 bs) o 
+      (ARM_WRITE_MEM a (EL 0 bs) o
        ARM_WRITE_MEM (a+1w) (EL 1 bs) o
        ARM_WRITE_MEM (a+2w) (EL 2 bs) o
        ARM_WRITE_MEM (a+3w) (EL 3 bs)) s`;
 
 val ARM_READ_NZCV_def = Define `
-  ARM_READ_NZCV s = 
+  ARM_READ_NZCV s =
     let cpsr = ARM_READ_CPSR s in
       (cpsr.N,cpsr.Z,cpsr.C,cpsr.V)`;
 
 val ARM_WRITE_NZCV_def = Define `
-  ARM_WRITE_NZCV (n,z,c,v) s = 
-    ARM_WRITE_CPSR 
-      (ARM_READ_CPSR s with <| N := n; Z := z; C := c; V := v |>) s`;  
+  ARM_WRITE_NZCV (n,z,c,v) s =
+    ARM_WRITE_CPSR
+      (ARM_READ_CPSR s with <| N := n; Z := z; C := c; V := v |>) s`;
 
 val eval_binop_def = Define `
   (eval_binop BINOP_ADD regs (n,z,c,v) = add_with_carry(regs 0w, regs 1w, F)) /\
@@ -131,9 +140,9 @@ val eval_binop_def = Define `
   (eval_binop BINOP_AND regs (n:bool,z:bool,c:bool,v:bool) = (regs 0w && regs 1w, c, v))`;
 
 val check_assert_def = Define `
-  (check_assert ASSERT_UNPREDICTABLE (regs:mini_reg -> word32) = F) /\ 
-  (check_assert ASSERT_NOT_IMPLEMENTED regs = F) /\ 
-  (check_assert ASSERT_ALIGNED_WORD regs = aligned (regs 0w, 2)) /\ 
+  (check_assert ASSERT_UNPREDICTABLE (regs:mini_reg -> word32) = F) /\
+  (check_assert ASSERT_NOT_IMPLEMENTED regs = F) /\
+  (check_assert ASSERT_ALIGNED_WORD regs = aligned (regs 0w, 2)) /\
   (check_assert ASSERT_ALIGNED_HALF regs = aligned (regs 0w, 1))`;
 
 
@@ -146,37 +155,39 @@ val check_assert_def = Define `
 
 val eval_mini_def = Define `
 
-  (eval_mini (MINI_CONDITIONAL cond) (regs,ok,s) = 
+  (eval_mini (MINI_CONDITIONAL cond imm) (regs,ok,s) =
      if arm_condition_passed cond (ARM_READ_NZCV s) then
        (F,regs,ok,s)
      else
-       (T,regs,ok,ARM_WRITE_REG 15w (ARM_READ_REG 15w s + 4w) s)) /\
-  (eval_mini (MINI_MARKER) (regs,ok,s) = (F,regs,ok,s)) /\ 
+       (T,regs,ok,ARM_WRITE_REG 15w (ARM_READ_REG 15w s + imm) s)) /\
+  (eval_mini (MINI_MARKER) (regs,ok,s) = (F,regs,ok,s)) /\
 
-  (eval_mini (MINI_MOVE a b) (regs,ok,s) = 
+  (eval_mini (MINI_MOVE a b) (regs,ok,s) =
      (F,(a =+ regs b) regs,ok,s)) /\
-  (eval_mini (MINI_IMM a imm32) (regs,ok,s) = 
+  (eval_mini (MINI_IMM a imm32) (regs,ok,s) =
      (F,(a =+ imm32) regs,ok,s)) /\
 
-  (eval_mini (MINI_REG_READ a r) (regs,ok,s) = 
+  (eval_mini (MINI_REG_READ a r) (regs,ok,s) =
      (F,(a =+ ARM_READ_REG r s) regs,ok,s)) /\
-  (eval_mini (MINI_REG_WRITE r a) (regs,ok,s) = 
+  (eval_mini (MINI_REG_WRITE r a) (regs,ok,s) =
      (F,regs,ok,ARM_WRITE_REG r (regs a) s)) /\
 
-  (eval_mini (MINI_MEM_BYTE_READ imm32) (regs,ok,s) = 
+  (eval_mini (MINI_MEM_BYTE_READ imm32) (regs,ok,s) =
      (F,(1w =+ w2w (ARM_READ_MEM (regs 0w + imm32) s)) regs,ok,s)) /\
-  (eval_mini (MINI_MEM_WORD_READ imm32) (regs,ok,s) = 
+  (eval_mini (MINI_MEM_WORD_READ imm32) (regs,ok,s) =
      (F,(1w =+ ARM_READ_MEM_WORD (regs 0w + imm32) s) regs,ok,s)) /\
-  (eval_mini (MINI_MEM_BYTE_WRITE imm32) (regs,ok,s) = 
+  (eval_mini (MINI_MEM_BYTE_WRITE imm32) (regs,ok,s) =
      (F,regs,ok,ARM_WRITE_MEM (regs 0w + imm32) (w2w (regs 1w)) s)) /\
-  (eval_mini (MINI_MEM_WORD_WRITE imm32) (regs,ok,s) = 
+  (eval_mini (MINI_MEM_WORD_WRITE imm32) (regs,ok,s) =
      (F,regs,ok,ARM_WRITE_MEM_WORD (regs 0w + imm32) (regs 1w) s)) /\
 
-  (eval_mini (MINI_ASSERT asrt) (regs,ok,s) = 
+  (eval_mini (MINI_ASSERT asrt) (regs,ok,s) =
      (F,regs,ok /\ check_assert asrt regs,s)) /\
 
+  (eval_mini (MINI_ADD_IMM a imm32) (regs,ok,s) =
+     (F,(a =+ regs a + imm32) regs,ok,s)) /\
   (eval_mini (MINI_BINOP binop s_flag) (regs,ok,s) =
-     let (res,c,v) = eval_binop binop regs (ARM_READ_NZCV s) in 
+     let (res,c,v) = eval_binop binop regs (ARM_READ_NZCV s) in
        (F,(0w =+ res) regs,ok,
         if s_flag then ARM_WRITE_NZCV (word_msb res,res = 0w,c,v) s else s))`;
 
@@ -187,21 +198,21 @@ val DROP_UNTIL_def = Define `
   (DROP_UNTIL p [] = []) /\
   (DROP_UNTIL p (x::xs) = if p x then x::xs else DROP_UNTIL p xs)`;
 
-val LENGTH_DROP_UNTIL = prove( 
+val LENGTH_DROP_UNTIL = prove(
   ``!xs. LENGTH (DROP_UNTIL P xs) <= LENGTH xs``,
   Induct THEN SRW_TAC [] [DROP_UNTIL_def] THEN DECIDE_TAC);
 
 val eval_mini_list_def = tDefine "eval_mini_list" `
   (eval_mini_list [] s = s) /\
-  (eval_mini_list (x::xs) s = 
+  (eval_mini_list (x::xs) s =
      let (stop,t) = eval_mini x s in
-       if stop then eval_mini_list (DROP_UNTIL (\x. x = MINI_MARKER) xs) t 
+       if stop then eval_mini_list (DROP_UNTIL (\x. x = MINI_MARKER) xs) t
                else eval_mini_list xs t)`
- (WF_REL_TAC `measure (LENGTH o FST)` 
+ (WF_REL_TAC `measure (LENGTH o FST)`
   THEN SIMP_TAC std_ss [LENGTH] THEN REPEAT STRIP_TAC
   THEN MATCH_MP_TAC LESS_EQ_LESS_TRANS THEN Q.EXISTS_TAC `LENGTH xs`
   THEN ASM_SIMP_TAC std_ss [LENGTH_DROP_UNTIL]);
 
-  
+
 val _ = export_theory();
 
